Update SkipList2.Insertion.fst

SkipList2/SkipList2.Insertion.fst
@@ -37,13 +37,74 @@ assume val change_indexes: #a : eqtype -> #f : cmp a -> sl:skipList a f {Sl.leng
 					} -> 
 					Tot(r: seq (non_empty_list nat) {Seq.length r = Sl.length sl + 1 })
 
+val sorted_seq_concat_wrapper : #a: eqtype -> f: cmp a ->pivot : a -> s1: seq a 
+			{Seq.sorted f s1 /\ (forall y. (Seq.mem y s1 ==> f y pivot))} ->  
+			s2: seq a {Seq.sorted f s2 /\ (forall y. (Seq.mem y s2 ==> f pivot y))}  ->
+		  Tot(s3: seq a{Seq.sorted f s3 /\ Seq.length s3 = Seq.length s1 + Seq.length s2 + 1}) 
 
-assume val change_values: #a: eqtype -> #f: cmp a -> sl: skipList a f {Sl.length sl > 0} -> value: a -> 
-					place: nat {place < Sl.length sl /\ 
-					f (Seq.index (getValues sl) place) value /\
-					(place = 0 \/ f(Seq.index (getValues sl) (place -1)) value = false)
-				} -> 
-					Tot (r: seq a {Seq.length r = Sl.length sl + 1 /\ Seq.sorted f r})
+let sorted_seq_concat_wrapper #a f pivot s1 s2 = 
+		let s3 = (Seq.append s1 (cons pivot s2)) in 
+		FStar.Seq.Properties.sorted_concat_lemma #a f s1 pivot s2; 
+		s3  
+
+assume val lemma_ch1:#a:eqtype -> f: cmp a ->  sl: skipList a f -> value : a -> 
+		 place: nat{ 
+				place < (Sl.length sl) /\
+				f (Seq.index (getValues sl) place) value /\
+				(place - 1 < 0 \/  f (Seq.index (getValues sl) (place-1)) value = false)} ->
+		 Lemma (ensures (
+		 	(Seq.sorted f (fst (Seq.split #a (Sl.getValues sl) place))) /\
+		 	(forall y. (Seq.mem y (fst (Seq.split #a (Sl.getValues sl) place))
+		 	==> f y value))))
+
+val lemma_ch1_wrapper: #a: eqtype -> f: cmp a -> sl: skipList a f -> value : a -> 
+				place: nat{ 
+				place < (Sl.length sl) /\
+				f (Seq.index (getValues sl) place) value /\
+				(place - 1 < 0 \/  f (Seq.index (getValues sl) (place-1)) value = false)} ->
+				Tot(s1: seq a { Seq.sorted f s1 /\
+				(forall y. (Seq.mem y (fst (Seq.split #a (Sl.getValues sl) place))==> f y value))})
+
+
+let lemma_ch1_wrapper #a f sl value place = 
+			let values = fst (Seq.split #a (Sl.getValues sl) place) in 
+			lemma_ch1 #a f sl value place; values				
+
+assume val lemma_ch2:#a:eqtype -> f: cmp a ->  sl: skipList a f -> value : a -> 
+		 place: nat{ 
+				place < (Sl.length sl) /\
+				f (Seq.index (getValues sl) place) value /\
+				(place - 1 < 0 \/  f (Seq.index (getValues sl) (place-1)) value = false)} ->
+		 Lemma (ensures (
+		 	(Seq.sorted f (snd (Seq.split #a (Sl.getValues sl) place))) /\
+		 	(forall y. (Seq.mem y (snd (Seq.split #a (Sl.getValues sl) place))
+		 	==> f value y))))
+
+val lemma_ch2_wrapper: #a: eqtype -> f: cmp a -> sl: skipList a f -> value : a -> 
+				place: nat{ 
+				place < (Sl.length sl) /\
+				f (Seq.index (getValues sl) place) value /\
+				(place - 1 < 0 \/  f (Seq.index (getValues sl) (place-1)) value = false)} ->
+				Tot(s1: seq a { Seq.sorted f s1 /\
+				(forall y. (Seq.mem y (snd (Seq.split #a (Sl.getValues sl) place))==> f value y))})
+
+let lemma_ch2_wrapper #a f sl value place = 
+			let values = snd (Seq.split #a (Sl.getValues sl) place) in 
+			lemma_ch2 #a f sl value place; values		
+
+val change_values: #a: eqtype -> f: cmp a -> sl: skipList a f -> value : a -> 
+		 place: nat{ 
+				place < (Sl.length sl) /\
+				f (Seq.index (getValues sl) place) value /\
+				(place - 1 < 0 \/  f (Seq.index (getValues sl) (place-1)) value = false)} ->
+		Tot(s3: seq a{Seq.sorted f s3 /\ 
+		Seq.length s3 = Sl.length sl+ 1 
+	}) 
+
+let change_values #a f sl value place = 
+	let s1 = lemma_ch1_wrapper #a f sl value place in 
+	let s2 = lemma_ch2_wrapper #a f sl value place in 
+	sorted_seq_concat_wrapper #a f value s1 s2 
 
 private val searchPlaceIndex: #a: eqtype -> #f: cmp a -> sl : skipList a f{Sl.length sl> 1} -> value: a-> 
 						counter_global: nat{counter_global < (Sl.length sl -1) /\ 
@@ -105,6 +166,6 @@ val addition: #a: eqtype -> #f: cmp a ->
 
 let addition #a #f sl value  = 
 	let place = searchPlace #a #f sl value in 
-	let values = change_values #a #f sl value place in 
+	let values = change_values #a f sl value place in 
 	let indexes = change_indexes #a #f sl value place in 
 	Mk values indexes 
